\documentclass[12pt]{article}
\usepackage{amsmath, amssymb, amsthm, tikz, pgfplots}
\usepackage{geometry, enumitem, mdframed, array, xcolor}
\geometry{margin=1in}

\newtheorem{definition}{Definition}
\newtheorem{theorem}{Theorem}
\newtheorem{method}{Method}
\newtheorem{example}{Example}
\newtheorem{lemma}{Lemma}
\newmdenv[linecolor=blue,linewidth=2pt]{keypoint}
\newmdenv[linecolor=red,linewidth=2pt]{warning}
\newmdenv[linecolor=green,linewidth=2pt]{insight}
\newmdenv[linecolor=purple,linewidth=2pt]{examtip}
\newmdenv[linecolor=orange,linewidth=2pt]{transformation}

\title{Lesson 20: Riccati to Second-Order Linear Transformation}
\author{ODE 1 - Prof. Adi Ditkowski}
\date{}

\begin{document}
\maketitle

\section{The Fundamental Transformation}

\begin{theorem}[Riccati to Second-Order Linear]
The Riccati equation
$$y' = q_0(x) + q_1(x)y + q_2(x)y^2$$
can be transformed into the second-order linear equation
$$u'' + p(x)u' + r(x)u = 0$$
via the substitution $y = -\frac{1}{q_2} \cdot \frac{u'}{u}$, where:
\begin{align}
p(x) &= -q_1 - \frac{q_2'}{q_2} \\
r(x) &= q_0 q_2
\end{align}
\end{theorem}

\begin{proof}
Starting with $y = -\frac{1}{q_2} \cdot \frac{u'}{u}$:

\begin{align}
y' &= -\frac{1}{q_2} \cdot \frac{d}{dx}\left(\frac{u'}{u}\right) + \frac{q_2'}{q_2^2} \cdot \frac{u'}{u} \\
&= -\frac{1}{q_2}\left(\frac{u''}{u} - \frac{(u')^2}{u^2}\right) + \frac{q_2'}{q_2^2} \cdot \frac{u'}{u} \\
&= -\frac{u''}{q_2 u} + \frac{1}{q_2} \cdot \frac{(u')^2}{u^2} + \frac{q_2'}{q_2^2} \cdot \frac{u'}{u} \\
&= -\frac{u''}{q_2 u} + \frac{1}{q_2} \cdot q_2^2 y^2 + \frac{q_2'}{q_2^2} \cdot (-q_2 y) \\
&= -\frac{u''}{q_2 u} + q_2 y^2 - \frac{q_2'}{q_2} y
\end{align}

Substituting into the Riccati equation and simplifying yields the stated result. $\square$
\end{proof}

\section{Alternative Transformation}

\begin{transformation}
\textbf{The Exponential Integral Approach:}

For the Riccati equation $y' = q_0 + q_1 y + q_2 y^2$, we can use:
$$v = \exp\left(\int y \, dx\right)$$

Then:
\begin{enumerate}
    \item $\frac{v'}{v} = y$ implies $y = \frac{v'}{v}$
    \item $y' = \frac{v''}{v} - \left(\frac{v'}{v}\right)^2 = \frac{v''}{v} - y^2$
    \item Substituting into Riccati: $\frac{v''}{v} - y^2 = q_0 + q_1 y + q_2 y^2$
    \item This gives: $v'' - q_1 v' - (1 + q_2)(v')^2/v + q_0 v = 0$
\end{enumerate}

This form is useful when $q_2 = -1$ as it simplifies to:
$$v'' - q_1 v' + q_0 v = 0$$
\end{transformation}

\section{Standard Examples}

\begin{example}[Constant Coefficients]
Solve: $y' = 1 + y^2$

\textbf{Method 1: Using $y = -u'/u$}

Here $q_0 = 1$, $q_1 = 0$, $q_2 = 1$. Since $q_2$ is constant, $q_2' = 0$.

The second-order equation becomes:
$$u'' + 0 \cdot u' + 1 \cdot u = 0 \implies u'' + u = 0$$

General solution: $u = c_1 \cos x + c_2 \sin x$

Therefore: $y = -\frac{u'}{u} = -\frac{-c_1 \sin x + c_2 \cos x}{c_1 \cos x + c_2 \sin x} = \frac{c_1 \sin x - c_2 \cos x}{c_1 \cos x + c_2 \sin x}$

Simplifying: $y = \tan(x - \phi)$ where $\tan \phi = c_2/c_1$
\end{example}

\begin{example}[Euler-Type Transformation]
Solve: $y' = \frac{a}{x^2} + b \cdot y^2$ where $a, b$ are constants.

Using $y = -\frac{1}{b} \cdot \frac{u'}{u}$ (note $q_2 = b$):

The second-order equation becomes:
$$u'' + 0 \cdot u' + \frac{ab}{x^2} u = 0$$

or equivalently:
$$x^2 u'' + ab \cdot u = 0$$

This is an Euler equation. Let $u = x^m$:
$$m(m-1) + ab = 0 \implies m = \frac{1 \pm \sqrt{1 - 4ab}}{2}$$

The nature of solutions depends on the discriminant $1 - 4ab$.
\end{example}

\section{Special Second-Order Forms}

\begin{keypoint}
\textbf{Common Transformations and Their Second-Order Forms:}
\begin{center}
\begin{tabular}{|l|l|}
\hline
\textbf{Riccati Form} & \textbf{Second-Order Result} \\
\hline
$y' = a + by^2$ (const) & $u'' + ab \cdot u = 0$ \\
$y' = \frac{a}{x^2} + by^2$ & $x^2u'' + ab \cdot u = 0$ (Euler) \\
$y' = ax^2 + by^2$ & $u'' + abx^2 u = 0$ (Airy-type) \\
$y' = q_0(x) - y^2$ & $u'' - q_0(x)u = 0$ \\
$y' = \frac{n(n+1)}{x^2} + y^2$ & Modified Bessel equation \\
\hline
\end{tabular}
\end{center}
\end{keypoint}

\begin{warning}
\textbf{When the Method Fails:}
\begin{itemize}
    \item If $q_2(x) = 0$ at some points, the transformation is singular there
    \item The resulting second-order equation may not have elementary solutions
    \item Series solutions or special functions may be required
    \item Numerical methods might be necessary for general $q_i(x)$
\end{itemize}
\end{warning}

\section{Reverse Transformation}

\begin{theorem}[Second-Order to Riccati]
Given the second-order linear equation:
$$u'' + p(x)u' + q(x)u = 0$$

The substitution $y = -\frac{u'}{u}$ yields the Riccati equation:
$$y' = -q(x) - p(x)y - y^2$$
\end{theorem}

\begin{insight}
\textbf{Why This Matters:}
\begin{itemize}
    \item Every linear second-order equation has an associated Riccati
    \item Solutions of one determine solutions of the other
    \item Qualitative properties transfer between the two forms
    \item Stability analysis can be done in either form
    \item Special functions defined by second-order equations give Riccati solutions
\end{itemize}
\end{insight}

\section{Solution Process Flowchart}

\begin{keypoint}
\textbf{Solution Process Algorithm:}
\begin{enumerate}
    \item Start with Riccati: $y' = q_0 + q_1y + q_2y^2$
    \item \textbf{If} you know a particular solution $y_p$:
    \begin{itemize}
        \item Use substitution $y = y_p + v$
        \item Solve resulting Bernoulli equation
    \end{itemize}
    \item \textbf{If} no particular solution is known:
    \begin{itemize}
        \item Use transformation $y = -\frac{u'}{q_2 u}$
        \item Solve resulting second-order linear equation
    \end{itemize}
    \item Back-substitute to find general solution
\end{enumerate}
\end{keypoint}

\section{Connection to Special Functions}

\begin{examtip}
\textbf{Prof. Ditkowski's Favorite Transformations:}
\begin{enumerate}
    \item Riccati $\to$ Constant coefficient: Usually solvable with exponentials
    \item Riccati $\to$ Euler equation: Power solutions
    \item Riccati $\to$ Airy equation: Special functions required
    \item Riccati $\to$ Bessel equation: Bessel functions needed
    \item Simple forms where $q_2 = \pm 1$: Often give nice solutions
\end{enumerate}
\end{examtip}

\end{document}