\documentclass[12pt]{article}
\usepackage{amsmath, amssymb, amsthm, geometry, enumitem}
\geometry{margin=1in}

\title{Lesson 44: Practice Problems\\Repeated Roots and $t$^{k}$$ Terms}
\author{ODE 1 with Prof. Adi Ditkowski}
\date{Tel Aviv University}

\usepackage{mdframed}
\usepackage{xcolor}
\usepackage{tikz}
\begin{document}

\maketitle

\section*{Part A: Identifying Multiplicities (5 problems)}

\begin{enumerate}
\item Given the characteristic polynomial $(r-3)^{2}(r+1) = 0$, identify all roots and their multiplicities.

\item Given the characteristic polynomial $r^{4} - 8r^{3} + 24r^{2} - 32r + 16 = 0$, show that it equals $(r-2)^{4}$ and identify the multiplicity.

\item The characteristic equation $(r^{2} - 2r + 5)^{2} = 0$ has complex roots. Find them and their multiplicities.

\item Factor completely: $r^{3} + 3r^{2} + 3r + 1 = 0$ and identify multiplicities.

\item Given $(r^{2} + 4)^{3} = 0$, identify all roots and multiplicities.
\end{enumerate}

\section*{Part B: Solutions from Multiplicities (5 problems)}

\begin{enumerate}[resume]
\item If $r = 3$ is a triple root, write all three linearly independent solutions.

\item If $r = -2$ has multiplicity 4, write the form of the general solution.

\item Complex roots $1 \pm 2i$ each have multiplicity 2. Write all four real solutions.

\item The characteristic polynomial is $(r+1)^{2}(r-2)^{3}$. Write the general solution.

\item If $\pm 3i$ are both double roots, write the general real solution.
\end{enumerate}

\section*{Part C: Complete ODEs with Repeated Roots (5 problems)}

\begin{enumerate}[resume]
\item Solve: $y'' - 6y' + 9y = 0$

\item Solve: $y''' + 3y'' + 3y' + y = 0$

\item Solve: $y^{(4)} - 4y''' + 6y'' - 4y' + y = 0$

\item Solve: $y'' + 4y' + 4y = 0$ with $y(0) = 2, y'(0) = -3$

\item Solve: $y^{(4)} + 4y'' + 4y = 0$
\end{enumerate}

\section*{Part D: Reduction of Order Applications (5 problems)}

\begin{enumerate}[resume]
\item Given that $y_{1} = $e^{-t$}$ solves $(D+1)^{2}[y] = 0$, use reduction of order to find $y_{2}$.

\item Verify that $t$e^{3t$}$ solves $y'' - 6y' + 9y = 0$ by direct substitution.

\item Show that if $y_{1} = $e^{rt$}$ solves $L[y] = 0$ where $r$ is a double root, then $y_{2} = t$e^{rt$}$ also solves it.

\item Given $y'' - 4y' + 4y = 0$ has solution $e^{2t}$, find the second solution using $y_{2} = v(t)$e^{2t$}$.

\item For the equation with characteristic polynomial $(r-a)^{3} = 0$, verify the Wronskian of $e^{at}, t$e^{at},$ t$^{2e}$^{at}$ is nonzero.
\end{enumerate}

\section*{Part E: Complex Repeated Roots (5 problems)}

\begin{enumerate}[resume]
\item Solve: $y^{(4)} + 8y'' + 16y = 0$

\item Find the general real solution when the characteristic polynomial is $(r^{2} + 2r + 2)^{2} = 0$.

\item Solve: $y^{(4)} + 4y''' + 8y'' + 8y' + 4y = 0$ (Hint: $(r^{2} + 2r + 2)^{2}$)

\item If $2 \pm 3i$ are both triple roots, how many linearly independent real solutions are there? List them.

\item Solve the IVP: $y'' + 2y' + 5y = 0$ with $y(0) = 0, y'(0) = 4$, given that $-1 \pm 2i$ are roots.
\end{enumerate}

\section*{Part F: Theoretical and Exam-Style Problems (5 problems)}

\begin{enumerate}[resume]
\item Prove that if $r_{0}$ is a root of multiplicity $m$ of the characteristic polynomial, then $p(r_{0}) = p'(r_{0}) = \cdots = p^{(m-1)}(r_{0}) = 0$ but $p^{(m)}(r_{0}) \neq 0$.

\item Show that the dimension of the solution space equals the degree of the differential equation, even with repeated roots.

\item A fourth-order equation has characteristic polynomial with roots: $r = 2$ (mult. 2), $r = -1$ (mult. 1), $r = 3$ (mult. 1). If a solution satisfies $y(0) = 1, y'(0) = 0, y''(0) = -1, y'''(0) = 2$, find it.

\item Explain why the functions $\{t$^{k}$ $e^{rt}$ : k = 0, 1, \ldots, m-1\}$ span the solution space for a root of multiplicity $m$.

\item (Prof. Ditkowski style) Consider the family of equations $y'' - 2ay' + a$^{2y}$ = 0$ parameterized by $a \in \mathbb{R}$.
\begin{enumerate}[label=(\alph*)]
\item Show that for all $a$, the characteristic equation has a repeated root.
\item Find the general solution in terms of $a$.
\item For which values of $a$ do all solutions remain bounded as $t \to \infty$?
\item Find the solution with $y(0) = 1, y'(0) = 0$.
\end{enumerate}
\end{enumerate}

\newpage

\section*{Solutions}

\subsection*{Part A: Identifying Multiplicities}

\begin{enumerate}
\item Roots: $r = 3$ (multiplicity 2), $r = -1$ (multiplicity 1)

\item Expand $(r-2)^{4} = r^{4} - 8r^{3} + 24r^{2} - 32r + 16$ $\checkmark$\\
Root: $r = 2$ (multiplicity 4)

\item $(r^{2} - 2r + 5)^{2} = 0 \Rightarrow r^{2} - 2r + 5 = 0$\\
$r = \frac{2 \pm \sqrt{4-20}}{2} = 1 \pm 2i$\\
Roots: $1 + 2i$ (mult. 2), $1 - 2i$ (mult. 2)

\item $r^{3} + 3r^{2} + 3r + 1 = (r+1)^{3} = 0$\\
Root: $r = -1$ (multiplicity 3)

\item $(r^{2} + 4)^{3} = 0 \Rightarrow r^{2} = -4 \Rightarrow r = \pm 2i$\\
Roots: $2i$ (mult. 3), $-2i$ (mult. 3)
\end{enumerate}

\subsection*{Part B: Solutions from Multiplicities}

\begin{enumerate}[resume]
\item $e^{3t}, t$e^{3t},$ t$^{2e}$^{3t}$

\item $y(t) = (c_{1} + c$_{2t}$ + c$_{3t}$^2 + c$_{4t}$^3)$e^{-2t$}$

\item Real solutions: $e$^{t}$\cos(2t), te$^{t}$\cos(2t), e$^{t}$\sin(2t), te$^{t}$\sin(2t)$

\item $y(t) = (c_{1} + c$_{2t}$)$e^{-t}$ + (c_{3} + c$_{4t}$ + c$_{5t}$^2)$e^{2t$}$

\item $y(t) = (c_{1} + c$_{2t}$)\cos(3t) + (c_{3} + c$_{4t}$)\sin(3t)$
\end{enumerate}

\subsection*{Part C: Complete ODEs with Repeated Roots}

\begin{enumerate}[resume]
\item Char. eq.: $r^{2} - 6r + 9 = (r-3)^{2} = 0$\\
Root: $r = 3$ (mult. 2)\\
General solution: $y(t) = (c_{1} + c$_{2t}$)$e^{3t$}$

\item Char. eq.: $r^{3} + 3r^{2} + 3r + 1 = (r+1)^{3} = 0$\\
Root: $r = -1$ (mult. 3)\\
General solution: $y(t) = (c_{1} + c$_{2t}$ + c$_{3t}$^2)$e^{-t$}$

\item Char. eq.: $(r-1)^{4} = 0$\\
Root: $r = 1$ (mult. 4)\\
General solution: $y(t) = (c_{1} + c$_{2t}$ + c$_{3t}$^2 + c$_{4t}$^3)e$^{t}$$

\item $(r+2)^{2} = 0$, so $y = (c_{1} + c$_{2t}$)$e^{-2t$}$\\
$y(0) = c_{1} = 2$\\
$y'(t) = c$_{2e}$^{-2t} - 2(c_{1} + c$_{2t}$)$e^{-2t$}$\\
$y'(0) = c_{2} - 2c_{1} = -3$\\
$c_{2} = 1$\\
Solution: $y(t) = (2 + t)$e^{-2t$}$

\item $r^{4} + 4r^{2} + 4 = (r^{2} + 2)^{2} = 0$\\
Roots: $\pm i\sqrt{2}$ (each mult. 2)\\
$y(t) = (c_{1} + c$_{2t}$)\cos(\sqrt{2}t) + (c_{3} + c$_{4t}$)\sin(\sqrt{2}t)$
\end{enumerate}

\subsection*{Part D: Reduction of Order Applications}

\begin{enumerate}[resume]
\item Let $y_{2} = v(t)$e^{-t$}$\\
Substituting into $(D+1)^{2}[y] = y'' + 2y' + y = 0$:\\
After simplification: $v'' = 0$\\
Thus $v = c$_{1t}$ + c_{2}$\\
Second solution: $y_{2} = t$e^{-t$}$

\item $y = t$e^{3t$}$\\
$y' = $e^{3t}$ + 3t$e^{3t}$ = (1 + 3t)$e^{3t$}$\\
$y'' = 3$e^{3t}$ + 3(1 + 3t)$e^{3t}$ = (6 + 9t)$e^{3t$}$\\
Substitute: $(6 + 9t)$e^{3t}$ - 6(1 + 3t)$e^{3t}$ + 9t$e^{3t$}$\\
$= $e^{3t}[6$ + 9t - 6 - 18t + 9t] = 0$ $\checkmark$

\item For double root $r$: $(D-r)^{2}[y] = 0$\\
If $y = t$e^{rt$}$: $y' = $e^{rt}$ + rt$e^{rt$}$\\
$y'' = 2r$e^{rt}$ + r$^{2te}$^{rt}$\\
$(D-r)^{2}[y] = D[(D-r)[t$e^{rt}]]$ = D[$e^{rt}]$ = r$e^{rt}$ - r$e^{rt}$ = 0$ $\checkmark$

\item $y_{2} = v(t)$e^{2t$}$\\
$y_{2}' = (v' + 2v)$e^{2t$}$\\
$y_{2}'' = (v'' + 4v' + 4v)$e^{2t$}$\\
Substituting: $e^{2t}[v'' + 4v' + 4v - 4v' - 8v + 4v] = $e^{2t}$ \cdot v'' = 0$\\
$v'' = 0 \Rightarrow v = c$_{1t}$ + c_{2}$\\
Second solution: $y_{2} = t$e^{2t$}$

\item $W = \begin{vmatrix} $e^{at}$ & t$e^{at}$ & t$^{2e}$^{at} \\ a$e^{at}$ & (1+at)$e^{at}$ & (2t+at^{2})$e^{at}$ \\ a$^{2e}$^{at} & (2a+a$^{2t}$)$e^{at}$ & (2+4at+a$^{2t}$^2)$e^{at}$ \end{vmatrix}$\\
After calculation: $W = 2$e^{3at}$ \neq 0$
\end{enumerate}

\subsection*{Part E: Complex Repeated Roots}

\begin{enumerate}[resume]
\item $(r^{2} + 4)^{2} = 0 \Rightarrow r = \pm 2i$ (each mult. 2)\\
$y(t) = (c_{1} + c$_{2t}$)\cos(2t) + (c_{3} + c$_{4t}$)\sin(2t)$

\item $r^{2} + 2r + 2 = 0 \Rightarrow r = -1 \pm i$\\
Each root has mult. 2\\
$y(t) = $e^{-t}[(c_{1}$ + c$_{2t}$)\cos(t) + (c_{3} + c$_{4t}$)\sin(t)]$

\item Roots: $-1 \pm i$ (each mult. 2)\\
$y(t) = $e^{-t}[(c_{1}$ + c$_{2t}$)\cos(t) + (c_{3} + c$_{4t}$)\sin(t)]$

\item 6 linearly independent real solutions:\\
$e^{2t}\cos(3t), t$e^{2t}\cos(3t),$ t$^{2e}$^{2t}\cos(3t)$\\
$e^{2t}\sin(3t), t$e^{2t}\sin(3t),$ t$^{2e}$^{2t}\sin(3t)$

\item Simple roots (not repeated): $r = -1 \pm 2i$\\
$y(t) = $e^{-t}[c_{1}\cos(2t)$ + c_{2}\sin(2t)]$\\
$y(0) = c_{1} = 0$\\
$y'(t) = $e^{-t}[-c_{1}\cos(2t)$ - c_{2}\sin(2t) - 2c_{1}\sin(2t) + 2c_{2}\cos(2t)]$\\
$y'(0) = -c_{1} + 2c_{2} = 4$\\
$c_{2} = 2$\\
Solution: $y(t) = 2$e^{-t}\sin(2t$)$
\end{enumerate}

\subsection*{Part F: Theoretical and Exam-Style Problems}

\begin{enumerate}[resume]
\item If $p(r) = (r - r_{0})$^{m}$ q(r)$ where $q(r_{0}) \neq 0$:\\
$p'(r) = m(r - r_{0})^{m-1}q(r) + (r - r_{0})$^{m}$ q'(r)$\\
At $r = r_{0}$: $p'(r_{0}) = 0$ if $m > 1$\\
Continue differentiating to show $p^{(k)}(r_{0}) = 0$ for $k < m$\\
But $p^{(m)}(r_{0}) = m! \cdot q(r_{0}) \neq 0$

\item Total number of solutions = sum of all multiplicities = degree of polynomial = order of ODE

\item Char. poly: $(r-2)^{2}(r+1)(r-3) = 0$\\
$y = (c_{1} + c$_{2t}$)$e^{2t}$ + c$_{3e}$^{-t} + c$_{4e}$^{3t}$\\
Apply initial conditions (solve 4\times4 system):\\
Final solution: $y(t) = (1 - \frac{2}{3}t)$e^{2t}$ + \frac{1}{4}$e^{-t}$ - \frac{1}{4}$e^{3t$}$

\item The operator $(D-r)$^{m}$$ has an $m$-dimensional kernel. The functions $t$^{k}$ $e^{rt$}$ for $k = 0, \ldots, m-1$ are linearly independent (nonzero Wronskian) and all satisfy $(D-r)$^{m}$[y] = 0$.

\item
\begin{enumerate}[label=(\alph*)]
\item Char. eq.: $r^{2} - 2ar + a^{2} = (r-a)^{2} = 0$\\
Always a double root at $r = a$

\item $y(t) = (c_{1} + c$_{2t}$)$e^{at$}$

\item Bounded as $t \to \infty$ only if $a \leq 0$

\item $y(0) = c_{1} = 1$\\
$y'(t) = c$_{2e}$^{at} + a(c_{1} + c$_{2t}$)$e^{at$}$\\
$y'(0) = c_{2} + ac_{1} = 0$\\
$c_{2} = -a$\\
Solution: $y(t) = (1 - at)$e^{at$}$
\end{enumerate}
\end{enumerate}

\end{document}