\documentclass[12pt]{article}
\usepackage{amsmath, amssymb, amsthm, tikz, pgfplots}
\usepackage{geometry, enumitem, mdframed, array, xcolor}
\geometry{margin=1in}

\newtheorem{definition}{Definition}
\newtheorem{theorem}{Theorem}
\newtheorem{method}{Method}
\newtheorem{example}{Example}
\newmdenv[linecolor=blue,linewidth=2pt]{keypoint}
\newmdenv[linecolor=red,linewidth=2pt]{warning}
\newmdenv[linecolor=green,linewidth=2pt]{insight}
\newmdenv[linecolor=purple,linewidth=2pt]{examtip}
\newmdenv[linecolor=orange,linewidth=2pt]{transformation}

\title{Lesson 18: Bernoulli Differential Equations}
\author{ODE 1 - Prof. Adi Ditkowski}
\date{}

\begin{document}
\maketitle

\section{Definition and Recognition}

\begin{definition}[Bernoulli Equation]
A Bernoulli differential equation has the form:
$$\frac{dy}{dx} + p(x)y = q(x)y^n$$
where $p(x)$ and $q(x)$ are continuous functions and $n \neq 0, 1$.
\end{definition}

\begin{keypoint}
\textbf{Why $n \neq 0, 1$?}
\begin{itemize}
    \item If $n = 0$: $y' + p(x)y = q(x)$ is already linear
    \item If $n = 1$: $y' + p(x)y = q(x)y$ gives $y' = y(q(x) - p(x))$, which is separable
    \item For all other $n$: The equation is genuinely nonlinear and requires the Bernoulli transformation
\end{itemize}
\end{keypoint}

\section{The Bernoulli Transformation}

\begin{transformation}
\textbf{The Power Substitution Method:}
\begin{enumerate}
    \item Given: $\frac{dy}{dx} + p(x)y = q(x)y^n$ with $n \neq 0, 1$
    \item Substitute: $v = y^{1-n}$
    \item Then: $y = v^{\frac{1}{1-n}}$ and $\frac{dy}{dx} = \frac{1}{1-n}v^{\frac{n}{1-n}} \cdot \frac{dv}{dx}$
    \item Alternatively: $\frac{dv}{dx} = (1-n)y^{-n} \cdot \frac{dy}{dx}$
    \item The transformed equation becomes:
    $$\frac{dv}{dx} + (1-n)p(x)v = (1-n)q(x)$$
    \item This is linear in $v$! Solve using integrating factor method
    \item Back-substitute: $y = v^{\frac{1}{1-n}}$
\end{enumerate}
\end{transformation}

\begin{warning}
\textbf{Critical Algebraic Steps:}
Starting from $v = y^{1-n}$:
\begin{align}
\frac{dv}{dx} &= (1-n)y^{-n} \frac{dy}{dx} \\
\frac{dy}{dx} &= \frac{y^n}{1-n} \frac{dv}{dx} \\
\end{align}
Substituting into the original equation and multiplying by $(1-n)y^{-n}$ gives the linear form.
\end{warning}

\section{Detailed Derivation}

\begin{theorem}[Bernoulli to Linear Transformation]
The substitution $v = y^{1-n}$ transforms the Bernoulli equation into a linear equation.

\textbf{Proof:}
\begin{align}
\text{Given: } & y' + p(x)y = q(x)y^n \\
\text{Let: } & v = y^{1-n} \\
\text{Then: } & \frac{dv}{dx} = (1-n)y^{-n}\frac{dy}{dx} \\
\text{So: } & \frac{dy}{dx} = \frac{y^n}{1-n}\frac{dv}{dx} \\
\text{Substitute: } & \frac{y^n}{1-n}\frac{dv}{dx} + p(x)y = q(x)y^n \\
\text{Multiply by } \frac{1-n}{y^n}: & \frac{dv}{dx} + (1-n)p(x)y^{1-n} = (1-n)q(x) \\
\text{Since } v = y^{1-n}: & \frac{dv}{dx} + (1-n)p(x)v = (1-n)q(x) \quad \square
\end{align}
\end{theorem}

\section{Standard Examples}

\begin{example}[Basic Bernoulli]
Solve: $y' + \frac{2y}{x} = x^2y^3$

\textbf{Solution:}
\begin{enumerate}
    \item Identify: $p(x) = \frac{2}{x}$, $q(x) = x^2$, $n = 3$
    \item Substitute: $v = y^{1-3} = y^{-2}$
    \item Transform: $\frac{dv}{dx} + (1-3)\frac{2v}{x} = (1-3)x^2$
    \item Simplify: $\frac{dv}{dx} - \frac{4v}{x} = -2x^2$
    \item Integrating factor: $\mu = e^{\int 4/x \, dx} = x^4$
    \item Multiply: $x^4\frac{dv}{dx} - 4x^3v = -2x^6$
    \item Integrate: $x^4v = -\frac{2x^7}{7} + C$
    \item Solve for $v$: $v = -\frac{2x^3}{7} + \frac{C}{x^4}$
    \item Back-substitute: $y^{-2} = -\frac{2x^3}{7} + \frac{C}{x^4}$
    \item Final: $y = \pm\left(-\frac{2x^3}{7} + \frac{C}{x^4}\right)^{-1/2}$
\end{enumerate}
\end{example}

\begin{example}[Logistic Equation]
Solve: $\frac{dP}{dt} = rP\left(1 - \frac{P}{K}\right)$ where $r, K > 0$

\textbf{Solution:}
\begin{enumerate}
    \item Expand: $\frac{dP}{dt} = rP - \frac{r}{K}P^2$
    \item Rearrange: $\frac{dP}{dt} - rP = -\frac{r}{K}P^2$ (Bernoulli with $n = 2$)
    \item Substitute: $v = P^{1-2} = P^{-1} = \frac{1}{P}$
    \item Transform: $\frac{dv}{dt} + rv = \frac{r}{K}$
    \item Solve linear equation: $v = \frac{1}{K} + Ce^{-rt}$
    \item Back-substitute: $P = \frac{1}{v} = \frac{K}{1 + CKe^{-rt}}$
    \item With initial condition $P(0) = P_0$: $P(t) = \frac{K}{1 + \left(\frac{K - P_0}{P_0}\right)e^{-rt}}$
\end{enumerate}
\end{example}

\section{Special Cases and Variations}

\begin{insight}
\textbf{Common Values of $n$ and Their Applications:}
\begin{center}
\begin{tabular}{|c|l|l|}
\hline
$n$ & Application & Substitution \\
\hline
$2$ & Logistic growth, Riccati connection & $v = y^{-1}$ \\
$3$ & Certain chemical reactions & $v = y^{-2}$ \\
$1/2$ & Fluid dynamics, heat transfer & $v = y^{1/2}$ \\
$-1$ & Inverse relationships & $v = y^2$ \\
$-2$ & Gravitational problems & $v = y^3$ \\
\hline
\end{tabular}
\end{center}
\end{insight}

\begin{examtip}
\textbf{Prof. Ditkowski's Exam Patterns:}
\begin{itemize}
    \item Often disguises Bernoulli equations - practice recognition
    \item Likes fractional powers: $n = 1/2, 3/2, -1/2$
    \item May combine with initial conditions
    \item Tests the connection to logistic growth
    \item Sometimes asks for qualitative behavior without full solution
    \item Partial credit for correct substitution identification
\end{itemize}
\end{examtip}

\section{Recognition Flowchart}

The key steps for recognizing and solving Bernoulli equations:

\begin{enumerate}
\item Check if the equation has form $y' + p(x)y = q(x)y^n$
\item If $n = 0$: Linear equation, use integrating factor
\item If $n = 1$: Separable equation
\item Otherwise: Apply Bernoulli substitution $v = y^{1-n}$
\end{enumerate}

\section{Solution Quality Check}

\begin{keypoint}
\textbf{Verification Steps:}
\begin{enumerate}
    \item Check that your transformed equation is truly linear
    \item Verify the integrating factor calculation
    \item Ensure back-substitution is algebraically correct
    \item Test with initial conditions if given
    \item Check for lost solutions when $y = 0$
\end{enumerate}
\end{keypoint}

\end{document}